theories/lang/cpp/logic/lifetime.v
@@ -7,16 +7,25 @@
  * Logical interpretation of object lifetime
  *)
 Require Import Coq.Lists.List.
-Require Import Coq.ZArith.BinInt.
-Require Import Coq.NArith.BinNatDef.
 
 From bedrock.lang.cpp Require Import ast semantics.
 From bedrock.lang.cpp.logic Require Import
-     pred path_pred heap_pred
-     translation_unit.
+     pred path_pred heap_pred.
+
+  Require Import bedrock.lang.cpp.heap_notations.
+  Local Open Scope bs_scope.
 
 Section with_cpp.
   Context `{Σ : cpp_logic} {σ : genv}.
+
+  (* wrap up [pred.vtable] as a [Rep] *)
+  (* note: [list globname] is problematic because i don't know where to
+   * start from. i can make this an [Offset], or i can simply add a [globname]
+   * for the starting class....
+   *)
+  Definition _vtable (q : Qp) (mp : list (obj_name * (ptr * Offset))) : Rep.
+    (* {| monPred_at p := vtable _ q p |}. *)
+  Admitted.
 
   (** this function computes a separation logic assertion that
     patches the virtual table of base classes with methods that have been
@@ -28,7 +37,7 @@ Section with_cpp.
       this would simplify some of the meta-theory, but it would complicate the
       proofs because in order to dispatch you need partial ownership of many
       tables.
-    
+
     note: because we don't have a well-foundedness condition on our environment,
     we use fuel to make this terminating. in practice this isn't a problem
     because the depth of the inheritence tree is bounded by the number of
@@ -36,29 +45,12 @@ Section with_cpp.
    *)
 
   (** * virtual function tables *)
-  (* wrap up [pred.vtable] as a [Rep] *)
-  Definition _vtable (q : Qp) (mp : gmap obj_name (ptr * list globname)) : Rep :=
-    {| monPred_at p := vtable mp q p |}.
 
   Require Import bedrock.avl.
 
   Definition patch := IM.t ptr.
-  Definition vt := list (obj_name * (ptr * list globname)).
-  Definition off := list globname.
-
-  (* this makes a vtable for a [Struct] treating it as the most derived class
-   *)
-  Definition make_vtable (σ : genv) (virt : list (obj_name * option obj_name))
-    : option vt :=
-    mapM (M:=option) (fun '(k,v) =>
-            match v with
-            | None => Some (k,(nullptr, nil))
-            | Some nm =>
-              match glob_addr σ nm with
-              | None => None
-              | Some p => Some (k, (p, nil))
-              end
-            end) virt.
+  Definition vt := list (obj_name * (ptr * Offset)).
+  Definition off := Offset.
 
   (* this patches a single vtable that already exists in memory.
    * [here_over] is the overrides of this class (which need to
@@ -73,28 +65,210 @@ Section with_cpp.
                        match over !! nm with
                        | Some to' =>
                          ((nm, (to', offset)) :: acc,
-                          match List.find (fun '(nm',_) => if decide (nm = nm') then true else false) here_over with
+                          match List.find (fun '(_, nm') => if decide (nm = nm') then true else false) here_over with
                           | None => over
-                          | Some (l,_) => <[ l := to.1 ]> over
+                          | Some (l,_) => <[ l := to' ]> over
                           end)
                        | None => ((nm, to) :: acc, over)
                        end) (nil, over) mp).
   Defined.
 
   Eval compute in fun p =>
-    update_vtable {[ "a"%bs := p ]} ("z"%bs::nil) nil (("a"%bs, (nullptr, nil)) :: nil).
+    update_vtable {[ "a"%bs := p ]} (_id) nil (("a"%bs, (nullptr, _id)) :: nil).
+
+  Fixpoint patch_vtables (fuel : nat) (this : Loc) (cls : globname) (o : off) (p : patch) (Q : mpred) {struct fuel} : mpred.
+  refine
+    match fuel with
+    | O => lfalse
+    | S fuel =>
+      match σ.(genv_tu) !! cls with
+      | Some (Gstruct st) =>
+        Exists v, _at this (_vtable 1 v) **
+                (let '(v',p') := update_vtable p o st.(s_overrides) v in
+                 _at this (_vtable 1 v') -*
+                     List.fold_right (fun '(cls',_) Q => patch_vtables fuel (_offsetL (_base σ cls cls') this) cls' (_dot o (_derived σ cls' cls)) p' Q) Q st.(s_bases))
+      | _ => lfalse
+      end
+    end.
+  Defined.
+
+  (* this makes a vtable for a [Struct] treating it as the most derived class
+   *)
+  Definition make_vtable (s : Struct) : option vt :=
+    match s with
+    | {| s_virtuals := virt |} =>
+    mapM (M:=option) (fun '(k,v) =>
+            match v with
+            | None => Some (k,(nullptr, _id))
+            | Some nm =>
+              match glob_addr σ nm with
+              | None => None
+              | Some p => Some (k, (p, _id))
+              end
+            end) virt
+    end.
+
+  Definition lifetime_begin (this : Loc) (cls : globname) (Q : mpred) : mpred.
+  refine
+    match σ.(genv_tu) !! cls with
+    | Some (Gstruct s) =>
+    match make_vtable s with
+    | Some v =>
+      match mapM _ s.(s_overrides) with
+      | Some over =>
+        let over := list_to_map over in
+      this |-> _vtable 1 v -*
+      List.fold_right (fun '(cls',_) Q =>
+                         patch_vtables 100 (this ., _base σ cls cls') cls'
+                                       (_derived σ cls' cls) over Q) Q s.(s_bases)
+      | None => lfalse
+      end
+    | _ => lfalse
+    end
+    | _ => lfalse
+    end.
+  refine (fun '(f,o) =>
+            match List.find (fun '(nm',_) => if decide (o = nm') then true else false) v with
+            | Some (_,(p,_)) => Some (f, p)
+            | None => None
+            end).
+  Defined.
+
+  Definition lifetime_end (this : Loc) (cls : globname) (Q : mpred) : mpred.
+    
+
+End with_cpp.
+
+  Require Import bedrock.lang.cpp.parser.
+Definition module : translation_unit := 
+  Eval reduce_translation_unit in parser.decls (
+    (Dstruct "_Z1A" (Some
+        {| s_bases := (nil)
+         ; s_fields :=
+          (nil)
+
+         ; s_layout := Unspecified
+         ; s_size := 8
+         ; s_virtuals := mk_virtuals
+          (("_ZNK1A3fooEv", None) :: ("_ZN1AD0Ev",
+            (Some "_ZN1AD0Ev")) :: nil)
+           ; s_overrides := mk_overrides
+            (nil)
+           ; s_virtual_dtor :=
+          (Some "_ZN1AD0Ev")|})) ::
+      (Dstruct "_Z1B" (Some
+          {| s_bases := (("_Z1A", {| li_offset :=0|}) :: nil)
+           ; s_fields :=
+            (nil)
+
+           ; s_layout := Unspecified
+           ; s_size := 8
+           ; s_virtuals := mk_virtuals
+            (("_ZN1BD0Ev",
+              (Some "_ZN1BD0Ev")) :: nil)
+             ; s_overrides := mk_overrides
+              (("_ZN1AD0Ev", "_ZN1BD0Ev") :: nil)
+             ; s_virtual_dtor :=
+            (Some "_ZN1BD0Ev")|})) ::
+        (Dstruct "_Z1C" (Some
+            {| s_bases := (("_Z1B", {| li_offset :=0|}) :: nil)
+             ; s_fields :=
+              (nil)
+
+             ; s_layout := Unspecified
+             ; s_size := 8
+             ; s_virtuals := mk_virtuals
+              (("_ZNK1C3fooEv",
+                (Some "_ZNK1C3fooEv")) :: ("_ZN1CD0Ev",
+                (Some "_ZN1CD0Ev")) :: nil)
+               ; s_overrides := mk_overrides
+                (("_ZNK1A3fooEv", "_ZNK1C3fooEv") :: ("_ZN1BD0Ev", "_ZN1CD0Ev") :: nil)
+               ; s_virtual_dtor :=
+              (Some "_ZN1CD0Ev")|}))
+        :: nil)%bs.
+
+  Eval compute in fun p => make_vtable (σ:={| genv_tu := module ; glob_addr := fun f => Some (p f) ; pointer_size := 8 |})
+  ({| s_bases := (("_Z1B", {| li_offset :=0|}) :: nil)
+             ; s_fields :=
+              (nil)
+
+             ; s_layout := Unspecified
+             ; s_size := 8
+             ; s_virtuals := mk_virtuals
+              (("_ZNK1C3fooEv",
+                (Some "_ZNK1C3fooEv")) :: ("_ZN1CD0Ev",
+                (Some "_ZN1CD0Ev")) :: nil)
+               ; s_overrides := mk_overrides
+                (("_ZNK1A3fooEv", "_ZNK1C3fooEv") :: ("_ZN1BD0Ev", "_ZN1CD0Ev") :: nil)
+               ; s_virtual_dtor :=
+              (Some "_ZN1CD0Ev")|})%bs.
+
+
+  Goal forall `{Σ : cpp_logic} (this : Loc) p Q,
+      let σ := {| genv_tu := module ; glob_addr := fun f => Some (p f) ; pointer_size := 8 |} in
+      let c := this in
+      let b := c ., _base σ "_Z1C" "_Z1B" in
+      let a := b ., _base σ "_Z1B" "_Z1A" in
+      |-- lifetime_begin a "_Z1A" (lifetime_begin b "_Z1B" (lifetime_begin c "_Z1C" Q)).
+    intros.
+    Require Import iris.proofmode.tactics.
+    (* unfold lifetime_begin; simpl. *)
+    iIntros "A".
+    simpl.
+    iIntros "B".
+    simpl.
+    iExists _. iSplitL "A"; [ iAssumption | ].
+    simpl.
+    iIntros "A".
+    iIntros "C".
+    simpl.
+    iExists _. iSplitL "B"; [ iAssumption | ].
+    simpl. iIntros "B".
+    iExists _. iSplitL "A"; [ iAssumption | ].
+    simpl.
+    iIntros "A".
+
+    A : B, C
+    B : virtual X
+    C : X
+
+
+  Require Import bedrock.lang.cpp.logic.wp.
+
+  Fixpoint to_path (ls : list globname) (g : globname) (loc : Loc) : Loc :=
+    match ls with
+    | nil => loc
+    | l :: ls =>
+      to_path ls l (_offsetL (_derived σ g l) loc)
+    end.
+
+
+
+
 
   (** this definition of [vtable] provides abstraction *)
   Definition vtable_def (q : Qp)
-             (s : gmap obj_name (thread_info -> list val -> (val -> epred) -> mpred))
-    : Rep :=
+             (s : list (obj_name * (thread_info -> list val -> (val -> epred) -> mpred)))
+    : Rep.
+  refine (
     as_Rep (fun this => Exists fps, (* abstraction *is* existential quantification *)
       _at (_eq this) (_vtable q fps) **
-      [∗map] n ↦ ps ∈ merge (fun a b => match a , b with
-                                     | Some a , Some b => Some (a,b)
-                                     | _ , _ => None
-                                     end) fps s ,
-      □ (Forall ti vs Q, snd ps ti vs Q -* fspec ti (Vptr (fst ps)) vs Q)).
+      [∗list] ps ∈ combine fps s,
+        let '((nm, (p,off)), (_, PQ)) := ps in
+        □ (Forall this ti vs Q,
+             PQ ti (Vptr this :: vs) Q -*
+             Exists this', to_path off _ (_eq this) &~ this' **
+             fspec ti (Vptr p) (Vptr this :: vs) Q))).
+     (** can this be dependent on σ? possibly because it won't matter what the
+         σ actually is.
+      *)
+  refine "???"%bs. (* todo: what do i fill in here? *)
+  Defined.
+
   Definition vtable_aux : seal (@vtable_def). by eexists. Qed.
   Definition vtable := vtable_aux.(unseal).
   Definition vtable_eq : @vtable = _ := vtable_aux.(seal_eq).
+
+
+End with_cpp.
+
