theories/lang/cpp/logic/pred.v
@@ -100,7 +100,7 @@ Module Type CPP_LOGIC.
           [ptr] to the type of the [this] argument of the method. For
           example, if you have 'B extends A' and B overrides a method of
           A, then A's vtable will contain a pointer to B's override and
-          the path ["A"] meaning that the function will act like a non-virtual
+          the path ["B"] meaning that the function will act like a non-virtual
           call to `static_cast<B*>(obj)`.
 
         note: technically, this list could just be a single [globname] because
@@ -110,7 +110,7 @@ Module Type CPP_LOGIC.
         note: we avoid using names in this definition because the caller
         may not have the most derived class in scope.
      *)
-    Parameter vtable : forall (mp : gmap obj_name (ptr * list globname)),
+    Parameter vtable : forall {σ : genv} (mp : list (obj_name * (ptr * (globname * list globname)))),
         Qp -> ptr -> mpred.
 
     (** the pointer points to the code
